# P3.1
$$MÂ·\ddot{y}(t) = F(t)-b\dot{y}(t)-ky(t)$$

(a)

$$y(t)=x_{1}(t),  \dot{y}=x_{2}(t)$$

(b)

$$\dot{x_{1}}(t)=\dot{y}(t)=x_{2}(t)$$

$$\dot{x_{2}}(t)=\ddot{y}(t)=-\frac{k}{M}x_{1}(t)-\frac{b}{M}x_{2}(t)+\frac{1}{M}F(t)$$

(c)

$$
x(t) =
\begin{pmatrix}
x_1(t) \\
x_2(t)
\end{pmatrix}
$$



$$
\dot{x}(t) =
\begin{bmatrix}
0 & 1 \\
-\frac{k}{M} & -\frac{b}{M}
\end{bmatrix}
x(t)
+
\begin{bmatrix}
0 \\
\frac{1}{M}
\end{bmatrix}
F(t)
$$


$$
y(t) =\begin{bmatrix}0 & 1\end{bmatrix}x(t)
$$

# P3.3

$$
x_1=i_L(t)\quad x_2=v_C(t)
$$

$$
\text{KVL: } -v_1(t)+L\frac{di_L(t)}{dt}-v_C(t)+v_2(t)=0
$$

$$
-v_1(t)+L\dot{x}_1(t)-x_2(t)+v_2(t)=0
$$

$$
\dot{x}_1=\frac{v_1(t)+x_2(t)-v_2(t)}{L}
$$

$$
\dot{x}_1=\frac{1}{L}x_2(t)+\frac{1}{L}v_1(t)-\frac{1}{L}v_2(t)
$$

$$
\text{KCL: } v_2(t)-v_C(t)=v_n
$$

$$
i_L(t)=\frac{v_n}{R}+i_C(t)
$$

$$
x_1(t)=\frac{v_2(t)-x_2(t)}{R}-C\frac{d v_C(t)}{dt}
$$

$$
C\dot{x}_2(t)=\frac{1}{R}v_2(t)-\frac{1}{R}x_2(t)-x_1(t)
$$

$$
\dot{x}_2(t)=-\frac{1}{C}x_1(t)-\frac{1}{RC}x_2(t)+\frac{1}{RC}v_2(t)
$$

$$
u(t)=
\begin{pmatrix}
v_1(t)\\
v_2(t)
\end{pmatrix}
$$

$$
\dot{x}(t)=
\left[
\begin{array}{cc}
0 & \frac{1}{L} \\
-\frac{1}{C} & -\frac{1}{RC}
\end{array}
\right]x(t)
+
\left[
\begin{array}{cc}
\frac{1}{L} & -\frac{1}{L} \\
0 & \frac{1}{RC}
\end{array}
\right]u(t)
$$

# P3.5
(a)

$$
G(s)=\frac{s+2}{s+8}\cdot\frac{1}{s-3}\cdot\frac{1}{s}
=\frac{s+2}{(s+8)(s-3)s}
$$

$$
T(s)=\frac{\dfrac{s+2}{(s+8)(s-3)s}}{1+\dfrac{s+2}{(s+8)(s-3)s}}
=\frac{s+2}{s^3+5s^2-23s+2}
$$

(b)

$$
r(t)=\begin{pmatrix}
x_1(t)\\x_2(t)\\x_3(t)
\end{pmatrix}
=\begin{pmatrix}
\dot{z}(t)\\\ddot{z}(t)\\\dddot{z}(t)
\end{pmatrix}
$$











